use reversed binary strings as fresh idents

compiler/src/compiler/StringNameGen.v
@@ -11,86 +11,145 @@ Local Open Scope string_scope.
 Local Open Scope char_scope.
 Local Open Scope N_scope.
 
-Local Axiom TODO_someone_freshnames: False.
-
 Definition maxLength: list string -> nat :=
   List.fold_right (fun s res => max res (String.length s)) 0%nat.
 
-Definition N_to_string(n: N): string := DecimalString.NilEmpty.string_of_uint (N.to_uint n).
+(* reversed binary string *)
+Fixpoint rev_binary_pos(p: positive): string :=
+  match p with
+  | xH => "1"
+  | xO q => String "0" (rev_binary_pos q)
+  | xI q => String "1" (rev_binary_pos q)
+  end.
 
-Lemma string_of_uint_inj: forall ui1 ui2,
-    NilEmpty.string_of_uint ui1 = NilEmpty.string_of_uint ui2 -> ui1 = ui2.
+Definition rev_binary(n: N): string :=
+  match n with
+  | N.pos p => rev_binary_pos p
+  | N0 => "0"
+  end.
+
+Lemma rev_binary_pos_nonempty: forall p,
+    rev_binary_pos p <> ""%string.
 Proof.
-  intros.
-  apply Option.eq_of_eq_Some.
-  rewrite <- (NilEmpty.usu ui1), <- (NilEmpty.usu ui2).
-  f_equal.
-  assumption.
+  destruct p; simpl; congruence.
 Qed.
 
-Lemma N_to_string_inj: forall n1 n2, N_to_string n1 = N_to_string n2 -> n1 = n2.
+Lemma rev_binary_pos_inj: forall p p',
+    rev_binary_pos p = rev_binary_pos p' ->
+    p = p'.
 Proof.
-  unfold N_to_string.
-  intros.
-  apply Unsigned.to_uint_inj.
-  apply string_of_uint_inj.
-  assumption.
+  induction p; intros; destruct p'; simpl in *; inversion H; try f_equal; eauto;
+    exfalso; eapply rev_binary_pos_nonempty; try eassumption; symmetry; eassumption.
 Qed.
 
-Lemma N_to_uint_nb_digits: forall e n,
-    10 ^ N.of_nat e <= n < 10 * 10 ^ N.of_nat e ->
-    Decimal.nb_digits (N.to_uint n) = S e.
+Lemma rev_binary_pos_non_zero: forall p,
+    rev_binary_pos p <> "0"%string.
+Proof.
+  destruct p; simpl; try congruence.
+  intro C. inversion C. eapply rev_binary_pos_nonempty. eassumption.
+Qed.
+
+Lemma rev_binary_inj: forall n n',
+    rev_binary n = rev_binary n' ->
+    n = n'.
 Proof.
   intros.
-  unfold N.to_uint.
-  destruct n.
-  - apply proj1 in H.
-    pose proof (N.pow_nonzero 10 (N.of_nat e)).
-    blia.
-  - unfold Pos.to_uint.
-    replace (Decimal.nb_digits (Decimal.rev (Pos.to_little_uint p))) with
-        (Decimal.nb_digits (Pos.to_little_uint p)) by admit.
-    revert dependent p.
-    induction e; intros.
-    + simpl in *.
-Abort.
+  destruct n; destruct n'; simpl in *.
+  - try reflexivity.
+  - symmetry in H. apply rev_binary_pos_non_zero in H. contradiction.
+  - apply rev_binary_pos_non_zero in H. contradiction.
+  - apply rev_binary_pos_inj in H. congruence.
+Qed.
 
-Lemma ten_to_number_of_digits_lower_bound: forall n,
-    n < 10 ^ N.of_nat (String.length (N_to_string n)).
+Lemma rev_binary_nonempty: forall n,
+    rev_binary n <> ""%string.
 Proof.
-  unfold N_to_string. intros.
-Admitted.
+  unfold rev_binary. intros. destruct n.
+  - congruence.
+  - apply rev_binary_pos_nonempty.
+Qed.
 
-Instance StringNameGen: NameGen string N. refine ({|
-  freshNameGenState(l: list string) := (10 ^ (N.of_nat (maxLength l)))%N;
-  genFresh(state: N) := (String "x" (N_to_string state), state + 1);
-  allFreshVars(state: N) := fun v => exists state', String "x" (N_to_string state') = v /\ state <= state';
-|}).
-(* TODO abstract proofs *)
-all: unfold PropSet.subset, PropSet.elem_of; intros.
-- inversion H; subst; clear H. ssplit.
-  + eexists. split; reflexivity.
-  + intro C. destruct C as [s' [E H]].
+Lemma two_to_number_of_digits_lower_bound: forall n,
+    n < 2 ^ N.of_nat (String.length (rev_binary n)).
+Proof.
+  intros. remember (rev_binary n) as s. revert dependent n.
+  induction s; intros.
+  - symmetry in Heqs. apply rev_binary_nonempty in Heqs. contradiction.
+  - destruct n.
+    + simpl in Heqs. inversion Heqs. subst. cbv. reflexivity.
+    + simpl in Heqs. destruct p.
+      * simpl in Heqs. inversion Heqs. subst.
+        change (String.length (String "1" (rev_binary_pos p))) with
+            (1 + (String.length (rev_binary_pos p)))%nat.
+        rewrite Nat2N.inj_add.
+        rewrite N.pow_add_r.
+        change (2 ^ N.of_nat 1) with 2.
+        change (N.pos p~1) with (1 + 2 * N.pos p).
+        specialize (IHs (N.pos p) eq_refl). blia.
+      * simpl in Heqs. inversion Heqs. subst.
+        change (String.length (String "0" (rev_binary_pos p))) with
+            (1 + (String.length (rev_binary_pos p)))%nat.
+        rewrite Nat2N.inj_add.
+        rewrite N.pow_add_r.
+        change (2 ^ N.of_nat 1) with 2.
+        change (N.pos p~1) with (1 + 2 * N.pos p).
+        specialize (IHs (N.pos p) eq_refl). blia.
+      * simpl in Heqs. inversion Heqs. subst.
+        cbv. reflexivity.
+Qed.
+
+Definition start_state(l: list string): N := 2 ^ N.of_nat (maxLength l).
+
+Definition fresh_string_var(state: N): string * N :=
+  (String "x" (rev_binary state), state + 1).
+
+Definition all_from(state: N): string -> Prop :=
+  fun v => exists state', String "x" (rev_binary state') = v /\ state <= state'.
+
+Lemma fresh_string_var_spec: forall (s s' : N) (x : string),
+    fresh_string_var s = (x, s') ->
+    PropSet.elem_of x (all_from s) /\
+    ~ PropSet.elem_of x (all_from s') /\
+    PropSet.subset (all_from s') (all_from s).
+Proof.
+  unfold fresh_string_var, all_from, PropSet.subset, PropSet.elem_of; intros.
+  inversion H; subst; clear H. ssplit.
+  - eexists. split; reflexivity.
+  - intro C. destruct C as [s' [E H]].
     inversion E. clear E.
-    apply N_to_string_inj in H1. blia.
-  + intros. destruct H as [s' [E H]]. subst x.
+    apply rev_binary_inj in H1. blia.
+  - intros. destruct H as [s' [E H]]. subst x.
     eexists. split; [reflexivity|]. blia.
-- intro C. destruct C as [state [E C]]. subst v.
+Qed.
+
+Lemma start_state_spec: forall (l : list string) (v : string),
+    In v l -> ~ PropSet.elem_of v (all_from (start_state l)).
+Proof.
+  unfold fresh_string_var, all_from, start_state, PropSet.subset, PropSet.elem_of; intros.
+  intro C. destruct C as [state [E C]]. subst v.
   revert dependent l. induction l; simpl; intros.
-  + assumption.
-  + destruct H.
-    * subst. simpl in *.
-      assert (10 ^ (N.of_nat (S (String.length (N_to_string state)))) <= state) as A. {
+  - assumption.
+  - destruct H.
+    + subst. simpl in *.
+      assert (2 ^ (N.of_nat (S (String.length (rev_binary state)))) <= state) as A. {
         eapply N.le_trans. 2: eassumption.
         apply N.pow_le_mono_r; blia.
       }
-      replace (N.of_nat (S (String.length (N_to_string state)))) with
-          (1 + N.of_nat (String.length (N_to_string state))) in A by blia.
+      replace (N.of_nat (S (String.length (rev_binary state)))) with
+          (1 + N.of_nat (String.length (rev_binary state))) in A by blia.
       rewrite N.pow_add_r in A.
-      change (10 ^ 1) with 10 in A.
-      pose proof (ten_to_number_of_digits_lower_bound state).
+      change (2 ^ 1) with 2 in A.
+      pose proof (two_to_number_of_digits_lower_bound state).
       blia.
-    * eapply IHl. 1: eassumption.
+    + eapply IHl. 1: eassumption.
       eapply N.le_trans. 2: eassumption.
       apply N.pow_le_mono_r; blia.
-Defined.
+Qed.
+
+Instance StringNameGen: NameGen string N := {|
+  freshNameGenState := start_state;
+  genFresh := fresh_string_var;
+  allFreshVars := all_from;
+  genFresh_spec := fresh_string_var_spec;
+  freshNameGenState_spec := start_state_spec;
+|}.
